tried (failed) to prove strong normalization for System-T

theories/SimplyTypedLambdaCalculus/StrongNormalisation.v
@@ -1,5 +1,5 @@
 From FormArith.SimplyTypedLambdaCalculus Require Import Definitions.
-
+From Coq Require Import  Lia .
 
 Inductive SN: term -> Prop :=
   | Strong (t: term) :
@@ -7,24 +7,37 @@ Inductive SN: term -> Prop :=
 
 Fixpoint reducible (A: type) (t: term): Prop :=
   match A with
-  | Base => SN t
+  | Base | Nat => SN t
   | Arr A B => forall (u: term), reducible A u -> reducible B (App t u)
   end.
 
 Definition neutral (t: term): Prop :=
   match t with
-  | Lam _ => False
+  | Lam _ | Const_0 | Const_S _ => False
   | _ => True
   end.
 
 Inductive sub_term: term -> term -> Prop :=
   | Sub_app1 (t1 t2: term) : sub_term t1 (App t1 t2)
   | Sub_app2 (t1 t2: term) : sub_term t2 (App t1 t2)
-  | Sub_lam (t: term) : sub_term t (Lam t).
-
+  | Sub_lam (t: term) : sub_term t (Lam t)
+  | Sub_S (s : term) : sub_term s (Const_S s)
+  | Sub_R0 (t0 ts n: term) : sub_term t0 (Rec t0 ts n)
+  | Sub_RS (t0 ts n: term) : sub_term ts (Rec t0 ts n).
 
 Lemma SN_lam (t: term):
   SN t -> SN (Lam t).
+Proof.
+  revert t.
+
+  apply SN_ind; intros ? _ H.
+  apply Strong; intros ? Hbeta.
+  inversion Hbeta; subst.
+  now apply H.
+Qed.
+
+Lemma SN_S (t: term):
+  SN t -> SN (Const_S t).
 Proof.
   revert t.
 
@@ -46,17 +59,36 @@ Proof.
        | H: _ |- _ => idtac
        end.
 
+  (* case: Sub_app1 *)
   - apply IH with (App u t2).
     + now apply Beta_AppL.
     + apply Sub_app1.
 
+  (* case: Sub_app2 *)
   - apply IH with (App t1 u).
     + now apply Beta_AppR.
     + apply Sub_app2.
 
+  (* case: Sub_lam *)
   - apply IH with (Lam u).
     + now apply Beta_Lam.
     + apply Sub_lam.
+
+  (* case: Sub_S *)
+  - apply IH with (Const_S u).
+    + now apply Beta_S.
+    + apply Sub_S.
+
+  (* case: Sub_R0 *)
+  - apply IH with (Rec u ts n).
+    + now apply Beta_RI0.
+    + apply Sub_R0.
+
+  (* case: Sub_R0 *)
+  - apply IH with (Rec t0 u n).
+    + now apply Beta_RIS.
+    + apply Sub_RS.
+
 Qed.
 
 Lemma SN_var_app (t: term) (n: var):
@@ -73,12 +105,25 @@ Proof.
   now inversion 1.
 Qed.
 
+
+
 Lemma reducible_is_SN (A : type):
   (forall (t: term), reducible A t -> SN t) /\
     (forall (t u: term), reducible A t -> t ~> u -> reducible A u) /\
     (forall (t: term), neutral t -> (forall (t': term), t ~> t' -> reducible A t') -> reducible A t).
 Proof.
-  induction A as [ | A [IHA1 [IHA2 IHA3]] B [IHB1 [IHB2 IHB3]] ].
+  induction A as [ | | A [IHA1 [IHA2 IHA3]] B [IHB1 [IHB2 IHB3]] ].
+  - do 3 split.
+    + intros.
+      apply SN_inverted with t'; [| assumption ].
+      now apply SN_inverted with t.
+
+    + intros.
+      apply SN_inverted with u; [| assumption ].
+      now apply SN_inverted with t.
+
+    + assumption.
+
   - do 3 split.
     + intros.
       apply SN_inverted with t'; [| assumption ].
@@ -120,6 +165,22 @@ Proof.
         now apply IHA2 with u.
 Qed.
 
+Lemma reducible_CR1 (A : type) (t: term): reducible A t -> SN t.
+Proof.
+apply reducible_is_SN.
+Qed.
+
+Lemma reducible_CR2 (A : type) (t u: term): reducible A t -> t ~> u -> reducible A u.
+Proof.
+apply reducible_is_SN.
+Qed.
+
+Lemma reducible_CR3 (A: type) (t: term):
+  neutral t -> (forall (t': term), t ~> t' -> reducible A t') -> reducible A t.
+Proof.
+apply reducible_is_SN.
+Qed.
+
 Lemma SN_subst (t: term) (σ: var -> term):
   SN t -> forall (u: term), t = u.[σ] -> SN u.
 Proof.
@@ -134,8 +195,11 @@ Proof.
 Qed.
 
 Lemma SN_ind_pair (P : term -> term -> Prop):
-  (forall t u, (forall t' u', ((t = t' /\ u ~> u') \/ (t ~> t' /\ u = u')) -> P t' u') -> P t u)
-    -> forall t u, SN t -> SN u -> P t u.
+  (forall t u,
+    (forall t' u', ((t = t' /\ u ~> u') \/ (t ~> t' /\ u = u'))
+                   -> P t' u')
+    -> P t u)
+  -> forall t u, SN t -> SN u -> P t u.
 Proof.
   intros IH ? ? Hsnt.
   revert u.
@@ -152,8 +216,57 @@ Proof.
     now apply Strong.
 Qed.
 
+Lemma SN_triple_ind (P : term -> term -> term -> Prop):
+    (forall s t u,
+      (forall s', s ~> s' -> P s' t u)
+      -> (forall t', t ~> t' -> P s t' u)
+      -> (forall u', u ~> u' -> P s t u') -> P s t u)
+    -> forall s t u, SN s -> SN t -> SN u -> P s t u.
+Proof.
+  intros IH s t u Hs.
+  revert t u. induction Hs as [s Hs1 Hs2].
+  apply Strong in Hs1.
+  intros t u Ht.
+  revert u. induction Ht as [t Ht1 Ht2].
+  apply Strong in Ht1.
+  intros u Hu. induction Hu as [u Hu1 Hu2].
+  apply Strong in Hu1.
+  apply IH.
+  - intros. apply Hs2. all: assumption.
+  - intros. apply Ht2. all: assumption.
+  - intros. apply Hu2. all: assumption.
+Qed.
+
+Lemma reducible_Rec (t0 ts n : term) (A: type):
+  reducible A t0 
+  -> reducible (Arr Nat (Arr A A)) ts
+  -> reducible Nat n
+  -> reducible A (Rec t0 ts n).
+Proof.
+intros Hrt0 Hrts Hrn.
+apply reducible_CR1 in Hrt0 as Hsnt0.
+apply reducible_CR1 in Hrts as Hsnts.
+apply reducible_CR1 in Hrn as Hsnn.
+revert Hrn Hrts Hrt0.
+apply SN_triple_ind with (s := t0) (t := ts) (u := n); [ | assumption .. ].
+clear Hsnt0 Hsnts Hsnn.
+clear t0 ts n.
+intros t0 ts n Ht0' Hts' Hn' Hn Hts Ht0.
+apply reducible_CR3; [now simpl |].
+inversion 1; subst.
+  - assumption.
+  - simpl in Hts. apply Hts.
+    ** apply SN_sub_term with (t := Const_S n0); [apply Hn | constructor].
+    ** admit.
+  - apply Ht0'. all: try assumption.
+    apply reducible_CR2 with (t := t0). all: assumption.
+  - apply Hts'. all: try assumption.
+    apply reducible_CR2 with (t := ts). all: assumption.
+Admitted.
+
 Lemma reducible_abs (v: term) (A B: type):
-  (forall (u: term), reducible A u -> reducible B v.[u/]) -> reducible (Arr A B) (Lam v).
+  (forall (u: term), reducible A u -> reducible B v.[u/]) 
+  -> reducible (Arr A B) (Lam v).
 Proof.
   intros Hred u Hredu.
   specialize (reducible_is_SN A) as [HA1 [HA2 HA3]].
@@ -198,12 +311,24 @@ Lemma reducible_var (A: type) (x: var) (Γ: var -> type):
 Proof.
   intros.
   destruct A.
-  - simpl.
-    apply Strong.
-    inversion 1.
+  - simpl. apply Strong. inversion 1.
+  - simpl. apply Strong. inversion 1.
   - apply reducible_is_SN; [ exact I |].
     inversion 1.
 Qed.
+
+Lemma size_recursion (X : Type) (sigma : X -> nat) (p : X -> Type) :
+  (forall x, (forall y, sigma y < sigma x -> p y) -> p x) ->
+  forall x, p x.
+Proof.
+  intros D x. apply D.
+  cut (forall n y, sigma y < n -> p y); [now eauto |].
+  clear x. intros n.
+  induction n; intros y E.
+  - exfalso. inversion E.
+  - apply D. intros x F. apply IHn. lia.
+Defined.
+
 
 Lemma typing_is_reducible (Γ: var -> type) (σ: var -> term):
   (forall (x: var), reducible (Γ x) (σ x)) ->
@@ -217,17 +342,33 @@ Proof.
   all: inversion 1; subst; simpl.
 
   - apply Hred.
+
   - apply IHt1 with (σ := σ) in H2; [| assumption ].
     apply IHt2 with (σ := σ) in H4; [| assumption ].
     now apply H2.
+
   - apply reducible_abs.
     intros u Hredu. asimpl.
     apply IHt with (A0 .: Γ); [| assumption ].
     intros [| x ]; simpl; [ assumption |].
     apply Hred.
+
+  (* case: Const_0 *)
+  - apply Strong. inversion 1.
+
+  (* case: Const_S *)
+  - specialize (IHt σ Nat Γ Hred H1).
+    simpl in IHt.
+    now apply SN_S.
+
+  (* case: Rec *)
+  - specialize (IHt1 σ A Γ Hred H3).
+    specialize (IHt2 σ (Arr Nat (Arr A A)) Γ Hred H5).
+    specialize (IHt3 σ Nat Γ Hred H6).
+    apply reducible_Rec. all: assumption.
 Qed.
 
-Corollary STLC_is_SN (A: type) (Γ: var -> type) (t: term):
+Corollary ST_is_SN (A: type) (Γ: var -> type) (t: term):
   Γ ⊢ t : A -> SN t.
 Proof.
   intros.
